WIP

code/ecdsap256/Hacl.Impl.P256.DH.fst
@@ -26,7 +26,7 @@ let ecp256dh_i c result scalar =
   let len = getCoordinateLenU64 c in 
   let scalarLen = getScalarLen c in 
 
-  let tempBuffer = create (size 30 *! len) (u64 0) in
+  let tempBuffer = create (size 20 *! len) (u64 0) in
     
   let resultBuffer = create (size 3 *! len) (u64 0) in
   let resultBufferX = sub resultBuffer (size 0) len in
@@ -36,6 +36,7 @@ let ecp256dh_i c result scalar =
   let resultY = sub result scalarLen scalarLen in
 
   secretToPublic #c resultBuffer scalar tempBuffer;
+
   let flag = isPointAtInfinityPrivate #c resultBuffer in
 
   let h0 = ST.get() in
@@ -102,7 +103,7 @@ let _ecp256dh_r #c result pubKey scalar =
   push_frame();
   admit();
   let len = getCoordinateLenU64 c in 
-  let tempBuffer = create (size 30 *! len) (u64 0) in
+  let tempBuffer = create (size 20 *! len) (u64 0) in
   let publicKeyBuffer = create (size 3 *! len) (u64 0) in
   bufferToJac #c pubKey publicKeyBuffer;
   let publicKeyCorrect = verifyQValidCurvePoint #c publicKeyBuffer tempBuffer in
