code/ecdsap256/Hacl.Impl.P256.PointDouble.fsti
@@ -12,24 +12,16 @@ open Hacl.Spec.P256.MontgomeryMultiplication
 open Spec.P256
 
 val point_double: #c: curve -> p: point c -> result: point c 
-  -> tempBuffer: lbuffer uint64  (getCoordinateLenU64 c *! 22ul) 
+  -> tempBuffer: lbuffer uint64  (getCoordinateLenU64 c *! 17ul) 
   -> Stack unit
     (requires fun h -> live h p /\ live h tempBuffer /\ live h result /\
       disjoint p tempBuffer /\ disjoint result tempBuffer /\
-      eq_or_disjoint p result /\
-      (
-	let prime = getPrime c in 
-	point_x_as_nat c h p < prime /\ 
-	point_y_as_nat c h p < prime /\
-	point_z_as_nat c h p < prime))
+      eq_or_disjoint p result /\ point_eval c h p)
   (ensures fun h0 _ h1 -> modifies (loc tempBuffer |+| loc result) h0 h1 /\  
     (
       let prime = getPrime c in 
       let len = getCoordinateLenU64 c in 
-      
-      point_x_as_nat c h1 result < prime /\ 
-      point_y_as_nat c h1 result < prime /\
-      point_z_as_nat c h1 result < prime /\ (
+      point_eval c h1 result /\ (
       
       let x, y, z = point_x_as_nat c h0 p, point_y_as_nat c h0 p, point_z_as_nat c h0 p in 
       let x3, y3, z3 = point_x_as_nat c h1 result, point_y_as_nat c h1 result, point_z_as_nat c h1 result in       
